lib/Buckets/PackedStringArrayMarshalling.i.dfy
@@ -1,0 +1,32 @@
+include "../Marshalling/GenericMarshalling.i.dfy"
+include "PackedStringArray"
+
+module PackedStringArrayMarshalling {
+  import opened PackedStringArray
+  import opened GenericMarshalling
+
+  function method grammar() : G
+  ensures ValidGrammar(PSAGrammar())
+  {
+    GTuple([
+      GUint32Array, // offsets
+      GbyteArray    // string bytes
+    ])
+  }
+
+  method toVal(psa: PSA.Psa)
+    returns (v: V)
+    requires PSA.WF(psa)
+    ensures ValidInGrammar(grammar(), v)
+  {
+    v := VTuple([VUint32Array(psa.offsets), VByteArray(psa.data)]);
+  }
+
+  method fromVal(v: V)
+    returns (psa: PSA.Psa)
+    requires ValidInGrammar(grammar(), v)
+    ensures PSA.WF(psa)
+  {
+    v := VTuple([VUint32Array(psa.offsets), VByteArray(psa.data)]);
+  }
+}
